src/Rupicola/Lib/NoExprReflection.v
@@ -3,15 +3,17 @@ Require Import Rupicola.Lib.Notations.
 Require Import Rupicola.Lib.Tactics.
 
 Section CompilerBasics.
-  Context {width: Z} {BW: Bitwidth width} {word: word.word width} {memT: map.map word Byte.byte}.
+  Context {width: Z} {BW: Bitwidth width}.
+  Local Notation word := (bits width).
+  Context {memT: map.map word Byte.byte}.
   Context {localsT: map.map String.string word}.
   Context {ext_spec: bedrock2.Semantics.ExtSpec}.
-  Context {word_ok : word.ok word} {mem_ok : map.ok memT}.
+  Context {mem_ok : map.ok memT}.
   Context {locals_ok : map.ok localsT}.
   Context {ext_spec_ok : Semantics.ext_spec.ok ext_spec}.
 
   Lemma compile_word_of_Z_constant {tr mem locals functions} (z: Z) :
-    let v := word.of_Z z in
+    let v := bits.of_Z width z in
     forall {P} {pred: P v -> predicate}
       {k: nlet_eq_k P v} {k_impl}
       var,
@@ -44,9 +46,9 @@ Section CompilerBasics.
          Memory := mem;
          Locals := locals;
          Functions := functions }>
-      cmd.seq (cmd.set var (expr.literal (word.unsigned w))) k_impl
+      cmd.seq (cmd.set var (expr.literal (Zmod.unsigned w))) k_impl
       <{ pred (nlet_eq [var] w k) }>.
-  Proof. repeat straightline; subst_lets_in_goal; rewrite word.of_Z_unsigned; eauto. Qed.
+  Proof. repeat straightline; subst_lets_in_goal; rewrite Zmod.of_Z_unsigned; eauto. Qed.
 
   Lemma compile_Z_constant {tr mem locals functions} z :
     let v := z in
@@ -56,7 +58,7 @@ Section CompilerBasics.
       (let v := v in
        <{ Trace := tr;
           Memory := mem;
-          Locals := map.put locals var (word.of_Z v);
+          Locals := map.put locals var (bits.of_Z width v);
           Functions := functions }>
        k_impl
        <{ pred (k v eq_refl) }>) ->
@@ -76,7 +78,7 @@ Section CompilerBasics.
       (let v := v in
        <{ Trace := tr;
           Memory := mem;
-          Locals := map.put locals var (word.of_Z (Z.of_nat v));
+          Locals := map.put locals var (bits.of_Z width (Z.of_nat v));
           Functions := functions }>
        k_impl
        <{ pred (k v eq_refl) }>) ->
@@ -140,42 +142,42 @@ Section CompilerBasics.
           exact (tm: t)) (only parsing).
 
   Definition compile_word_add :=
-    unfold_id (@compile_binop_xxx _ id bopname.add word.add ltac:(reflexivity)).
+    unfold_id (@compile_binop_xxx _ id bopname.add Zmod.add ltac:(reflexivity)).
   Definition compile_word_sub :=
-    unfold_id (@compile_binop_xxx _ id bopname.sub word.sub ltac:(reflexivity)).
+    unfold_id (@compile_binop_xxx _ id bopname.sub Zmod.sub ltac:(reflexivity)).
   Definition compile_word_mul :=
-    unfold_id (@compile_binop_xxx _ id bopname.mul word.mul ltac:(reflexivity)).
+    unfold_id (@compile_binop_xxx _ id bopname.mul Zmod.mul ltac:(reflexivity)).
   Definition compile_word_mulhuu :=
-    unfold_id (@compile_binop_xxx _ id bopname.mulhuu word.mulhuu ltac:(reflexivity)).
+    unfold_id (@compile_binop_xxx _ id bopname.mulhuu (fun x y => bits.of_Z width (Zmod.unsigned x * Zmod.unsigned y / 2 ^ width)) ltac:(reflexivity)).
   Definition compile_word_divu :=
-    unfold_id (@compile_binop_xxx _ id bopname.divu word.divu ltac:(reflexivity)).
+    unfold_id (@compile_binop_xxx _ id bopname.divu Zmod.udiv ltac:(reflexivity)).
   Definition compile_word_remu :=
-    unfold_id (@compile_binop_xxx _ id bopname.remu word.modu ltac:(reflexivity)).
+    unfold_id (@compile_binop_xxx _ id bopname.remu Zmod.umod ltac:(reflexivity)).
   Definition compile_word_and :=
-    unfold_id (@compile_binop_xxx _ id bopname.and word.and ltac:(reflexivity)).
+    unfold_id (@compile_binop_xxx _ id bopname.and Zmod.and ltac:(reflexivity)).
   Definition compile_word_or :=
-    unfold_id (@compile_binop_xxx _ id bopname.or word.or ltac:(reflexivity)).
+    unfold_id (@compile_binop_xxx _ id bopname.or Zmod.or ltac:(reflexivity)).
   Definition compile_word_xor :=
-    unfold_id (@compile_binop_xxx _ id bopname.xor word.xor ltac:(reflexivity)).
+    unfold_id (@compile_binop_xxx _ id bopname.xor Zmod.xor ltac:(reflexivity)).
   Definition compile_word_sru :=
-    unfold_id (@compile_binop_xxx _ id bopname.sru word.sru ltac:(reflexivity)).
+    unfold_id (@compile_binop_xxx _ id bopname.sru Semantics.sru ltac:(reflexivity)).
   Definition compile_word_slu :=
-    unfold_id (@compile_binop_xxx _ id bopname.slu word.slu ltac:(reflexivity)).
+    unfold_id (@compile_binop_xxx _ id bopname.slu Semantics.slu ltac:(reflexivity)).
   Definition compile_word_srs :=
-    unfold_id (@compile_binop_xxx _ id bopname.srs word.srs ltac:(reflexivity)).
+    unfold_id (@compile_binop_xxx _ id bopname.srs Semantics.srs ltac:(reflexivity)).
 
   Definition compile_Z_add :=
-    @compile_binop_xxx _ word.of_Z bopname.add Z.add word.ring_morph_add.
+    @compile_binop_xxx _ (Zmod.of_Z (2 ^ width)) bopname.add Z.add (Zmod.of_Z_add (m := 2 ^ width)).
   Definition compile_Z_sub :=
-    @compile_binop_xxx _ word.of_Z bopname.sub Z.sub word.ring_morph_sub.
+    @compile_binop_xxx _ (Zmod.of_Z (2 ^ width)) bopname.sub Z.sub (Zmod.of_Z_sub (m := 2 ^ width)).
   Definition compile_Z_mul :=
-    @compile_binop_xxx _ word.of_Z bopname.mul Z.mul word.ring_morph_mul.
+    @compile_binop_xxx _ (Zmod.of_Z (2 ^ width)) bopname.mul Z.mul (Zmod.of_Z_mul (m := 2 ^ width)).
   Definition compile_Z_and :=
-    @compile_binop_xxx _ word.of_Z bopname.and Z.land word.morph_and.
+    @compile_binop_xxx _ (Zmod.of_Z (2 ^ width)) bopname.and Z.land word.morph_and.
   Definition compile_Z_or :=
-    @compile_binop_xxx _ word.of_Z bopname.or Z.lor word.morph_or.
+    @compile_binop_xxx _ (Zmod.of_Z (2 ^ width)) bopname.or Z.lor word.morph_or.
   Definition compile_Z_xor :=
-    @compile_binop_xxx _ word.of_Z bopname.xor Z.lxor word.morph_xor.
+    @compile_binop_xxx _ (Zmod.of_Z (2 ^ width)) bopname.xor Z.lxor word.morph_xor.
 
   Lemma compile_binop_xxb {T} T2w op (f: T -> T -> bool)
         (H: forall x y, word.b2w (f x y) = Semantics.interp_binop op (T2w x) (T2w y))
@@ -203,36 +205,36 @@ Section CompilerBasics.
   Proof. repeat (eexists; split; eauto). Qed.
 
   Ltac compile_binop_wwb_t :=
-    unfold id; cbn; intros; destruct_one_match; reflexivity.
+    unfold id, Semantics.ltu, Semantics.lts; cbn; intros; destruct_one_match; reflexivity.
 
   Definition compile_word_lts :=
-    unfold_id (@compile_binop_xxb _ id bopname.lts word.lts ltac:(compile_binop_wwb_t)).
+    unfold_id (@compile_binop_xxb _ id bopname.lts Semantics.lts ltac:(compile_binop_wwb_t)).
   Definition compile_word_ltu :=
-    unfold_id (@compile_binop_xxb _ id bopname.ltu word.ltu ltac:(compile_binop_wwb_t)).
+    unfold_id (@compile_binop_xxb _ id bopname.ltu Semantics.ltu ltac:(compile_binop_wwb_t)).
   Definition compile_word_eqb :=
-    unfold_id (@compile_binop_xxb _ id bopname.eq word.eqb ltac:(compile_binop_wwb_t)).
+    unfold_id (@compile_binop_xxb _ id bopname.eq Zmod.eqb ltac:(compile_binop_wwb_t)).
 
   Lemma bool_word_eq_compat {T} (T2w: T -> word) (eqb: T -> T -> bool)
         (T2w_inj: forall x y, T2w x = T2w y -> x = y)
         (eqb_compat: forall x y, eqb x y = true <-> x = y) :
     forall x y,
       word.b2w (eqb x y) =
-      (if word.eqb (T2w x) (T2w y) then word.of_Z 1 else word.of_Z 0) :> word.
+      (if Zmod.eqb (T2w x) (T2w y) then Zmod.one else Zmod.zero) :> word.
   Proof.
-    intros; rewrite word.unsigned_eqb.
+    intros; unfold Zmod.eqb.
     destruct eqb eqn:Hb; destruct Z.eqb eqn:Hz; try reflexivity.
     - apply eqb_compat in Hb; subst.
       apply Z.eqb_neq in Hz; congruence.
-    - apply Z.eqb_eq, word.unsigned_inj, T2w_inj in Hz; subst.
+    - apply Z.eqb_eq, Zmod.unsigned_inj, T2w_inj in Hz; subst.
       rewrite (proj2 (eqb_compat _ _)) in Hb; congruence.
   Qed.
 
   Ltac compile_binop_bbb_t lemma :=
-    unfold word.b2w; intros x y; cbn;
+    intros x y; cbn -[word.b2w];
     match goal with
     | [  |- _ = ?w ] =>
-      rewrite <- (word.of_Z_unsigned w);
-      rewrite lemma, !word.unsigned_of_Z_b2z; destruct x, y; reflexivity
+      rewrite <- (Zmod.of_Z_unsigned w);
+      rewrite lemma, !word.unsigned_b2w; destruct x, y; reflexivity
     end.
 
   Notation cbv_beta_b2w x :=
@@ -250,15 +252,15 @@ Section CompilerBasics.
   Definition compile_bool_andb :=
     cbv_beta_b2w (@compile_binop_xxb
                     _ (fun x => word.b2w x) bopname.and andb
-                    ltac:(compile_binop_bbb_t word.unsigned_and_nowrap)).
+                    ltac:(compile_binop_bbb_t bits.unsigned_and)).
   Definition compile_bool_orb :=
     cbv_beta_b2w (@compile_binop_xxb
                     _ (fun x => word.b2w x) bopname.or orb
-                    ltac:(compile_binop_bbb_t word.unsigned_or_nowrap)).
+                    ltac:(compile_binop_bbb_t bits.unsigned_or)).
   Definition compile_bool_xorb :=
     cbv_beta_b2w (@compile_binop_xxb
                     _ (fun x => word.b2w x) bopname.xor xorb
-                    ltac:(compile_binop_bbb_t word.unsigned_xor_nowrap)).
+                    ltac:(compile_binop_bbb_t bits.unsigned_xor)).
 
   Lemma compile_copy_word {tr mem locals functions} v0 :
     let v := v0 in
