src/Rupicola/Lib/Conditionals.v
@@ -5,10 +5,12 @@ Require Import Rupicola.Lib.Compiler.
 Require Import Rupicola.Lib.Invariants.
 
 Section Conditionals.
-  Context {width: Z} {BW: Bitwidth width} {word: word.word width} {memT: map.map word Byte.byte}.
+  Context {width: Z} {BW: Bitwidth width}.
+  Local Notation word := (bits width).
+  Context {memT: map.map word Byte.byte}.
   Context {localsT: map.map String.string word}.
   Context {ext_spec: bedrock2.Semantics.ExtSpec}.
-  Context {word_ok : word.ok word} {mem_ok : map.ok memT}.
+  Context {mem_ok : map.ok memT}.
   Context {locals_ok : map.ok localsT}.
   Context {ext_spec_ok : Semantics.ext_spec.ok ext_spec}.
 
@@ -129,7 +131,7 @@ Ltac compile_if :=
 
 Section Examples.
   Context {width: Z} {BW: Bitwidth width}.
-  Context {word: word.word width} {word_ok : word.ok word}.
+  Local Notation word := (bits width).
   Context {locals: map.map string word} {locals_ok : map.ok locals}.
   Context {mem: map.map word byte} {mem_ok : map.ok mem}.
 
